Com_SIL.thy
@@ -9,7 +9,7 @@ datatype
       | Seq    com  com         (\<open>_;;/ _\<close>  [60, 61] 60)
       | If     bexp com com     (\<open>(IF _/ THEN _/ ELSE _)\<close>  [0, 0, 61] 61)
       | SelectND " (bexp  \<times> com) list" (\<open>SELECT _\<close> [0] 61)
-      | ChoiceND "com list" (\<open>CHOICE _ ]\<close> [0] 61)
+     (* | ChoiceND "com list" (\<open>CHOICE _ ]\<close> [0] 61) *)
       | While  bexp com         (\<open>(WHILE _/ DO _)\<close>  [0, 61] 61)
 
 end
