SIL.thy
@@ -49,8 +49,14 @@ tSelectND: "\<lbrakk>\<forall>s. P s \<longrightarrow> (
    \<Longrightarrow> \<turnstile> \<langle>P\<rangle> SELECT bs \<langle>Q\<rangle>" |
 *)
 
-tSelectND: "\<lbrakk>\<forall>b c. (b,c) \<in> set bs \<and> \<turnstile> \<langle>\<lambda>s. (P b c) s \<and> bval b s\<rangle> c \<langle>Q\<rangle>\<rbrakk>
-   \<Longrightarrow> \<turnstile> \<langle>\<Or> {(P b c) | b c. (b,c) \<in> set bs }\<rangle> SELECT bs \<langle>Q\<rangle>" |
+tSelectND: "
+\<lbrakk>
+  \<forall>bc \<in> set bs. case bc of (b,c) \<Rightarrow>
+  (\<turnstile> \<langle>\<lambda>s. (R b c) s \<and> bval b s\<rangle> c \<langle>Q\<rangle>);
+  \<forall>s. P s \<longrightarrow> (\<exists>b c.(b, c) \<in> set bs 
+  \<and> (R b c) s \<and> bval b s)
+\<rbrakk>
+   \<Longrightarrow> \<turnstile> \<langle>P\<rangle> SELECT bs \<langle>Q\<rangle>" |
 
 (*
 tSelectND: "\<lbrakk>
